vera/VerilogSMT.v
@@ -5,7 +5,7 @@ From Stdlib Require Import List.
 From Stdlib Require Import Logic.FunctionalExtensionality.
 From Stdlib Require Import Logic.ProofIrrelevance.
 From Stdlib Require Import Structures.Equalities.
-Import ListNotations.
+From Stdlib Require Import Morphisms.
 
 From Equations Require Import Equations.
 
@@ -22,6 +22,9 @@ From vera Require Import BVList.
 Import BITVECTOR_LIST.
 
 From vera Require SMTLib.
+
+Import ListNotations.
+Local Open Scope list.
 
 Import SigTNotations.
 
@@ -103,122 +106,351 @@ Module VerilogSMTBijection.
   Qed.
 End VerilogSMTBijection.
 
-Module SMT.
-  Import VerilogSMTBijection (bij_inverse, bij_apply, bij_wf).
-  Import (coercions) VerilogSMTBijection.
+Import VerilogSMTBijection (bij_inverse, bij_apply, bij_wf).
+Import (coercions) VerilogSMTBijection.
 
-  Definition match_map_vars (tag : TaggedVariable.Tag) (map : VerilogSMTBijection.t) vars :=
-    forall var, (exists smtName, map (tag, var) = Some smtName) <-> (In var vars).
+Definition match_map_vars (tag : TaggedVariable.Tag) (map : VerilogSMTBijection.t) vars :=
+  forall var, (exists smtName, map (tag, var) = Some smtName) <-> (In var vars).
 
-  Record smt_with_namemap :=
-    MkSMTWithNameMap
-      { query : SMTQueries.query;
-        nameMap : VerilogSMTBijection.t;
-      }.
+Record smt_with_namemap :=
+  MkSMTWithNameMap
+    { assertions : SMTQueries.query;
+      nameMap : VerilogSMTBijection.t;
+    }.
 
-  Definition max_declaration (q : SMTQueries.query) : nat :=
-    List.list_max (SMTQueries.domain q).
+Definition max_declaration (q : SMTQueries.query) : nat :=
+  List.list_max (SMTQueries.domain q).
 
-  Lemma max_declaration_domain q name :
-    In name (SMTQueries.domain q) ->
-    name <= max_declaration q.
-  Proof.
-    unfold max_declaration, SMTQueries.domain.
-    revert name. rewrite <- Forall_forall.
-    apply list_max_le.
-    trivial.
-  Qed.
+Lemma max_declaration_domain q name :
+  In name (SMTQueries.domain q) ->
+  name <= max_declaration q.
+Proof.
+  unfold max_declaration, SMTQueries.domain.
+  revert name. rewrite <- Forall_forall.
+  apply list_max_le.
+  trivial.
+Qed.
 
-  Equations default (s : SMTLib.sort) : SMTLib.interp_sort s :=
-    default (SMTLib.Sort_Bool) := false;
-    default (SMTLib.Sort_BitVec n) := BV.zeros n.
+Equations default (s : SMTLib.sort) : SMTLib.interp_sort s :=
+  default (SMTLib.Sort_Bool) := false;
+  default (SMTLib.Sort_BitVec n) := BV.zeros n.
 
-  Import EqNotations.
+Import EqNotations.
 
-  Definition execution_of_valuation (tag : TaggedVariable.Tag) (m : VerilogSMTBijection.t) (ρ : SMTLib.valuation) : execution :=
-    fun var =>
-      match m (tag, var) with
-      | Some smtName => XBV.from_bv (ρ (SMTLib.Sort_BitVec (Verilog.varType var)) smtName)
-      | None => XBV.exes _
-      end
-  .
+Definition execution_of_valuation (tag : TaggedVariable.Tag) (m : VerilogSMTBijection.t) (ρ : SMTLib.valuation) : execution :=
+  fun var =>
+    match m (tag, var) with
+    | Some smtName => XBV.from_bv (ρ (SMTLib.Sort_BitVec (Verilog.varType var)) smtName)
+    | None => XBV.exes _
+    end
+.
 
-  Lemma execution_of_valuation_defined_value tag (m : VerilogSMTBijection.t) ρ:
-    RegisterState.defined_value_for
-      (fun var => exists smtName, m (tag, var) = Some smtName)
-      (SMT.execution_of_valuation tag m ρ).
-  Proof.
-    unfold SMT.execution_of_valuation.
-    intros var [smtName Hvar].
-    rewrite Hvar.
+Lemma execution_of_valuation_defined_value tag (m : VerilogSMTBijection.t) ρ:
+  RegisterState.defined_value_for
+    (fun var => exists smtName, m (tag, var) = Some smtName)
+    (execution_of_valuation tag m ρ).
+Proof.
+  unfold execution_of_valuation.
+  intros var [smtName Hvar].
+  rewrite Hvar.
+  eauto.
+Qed.
+
+Definition valuation_of_executions (m : VerilogSMTBijection.t) (e1 e2 : execution) : SMTLib.valuation :=
+  fun s smtName =>
+    match s as s' return SMTLib.interp_sort s' with
+    | SMTLib.Sort_Bool => default _
+    | SMTLib.Sort_BitVec w => 
+      match bij_inverse m smtName with
+| None => default _
+| Some (tag, verilogVar) =>
+  match dec (Verilog.varType verilogVar = w) with
+  | right _ => default _
+  | left E =>
+          let e :=
+            match tag with
+            | TaggedVariable.VerilogLeft => e1
+            | TaggedVariable.VerilogRight => e2
+            end
+          in
+            match XBV.to_bv (e verilogVar) with
+            (* TODO: Fix handling of Xs *)
+            | None => default _
+            | Some val => rew E in val
+            end
+  end
+end
+    end.
+
+Lemma execution_of_valuation_left_match_on (m : VerilogSMTBijection.t) e1 e2 l :
+  RegisterState.defined_value_for (fun var => In var l) e1 ->
+  match_map_vars TaggedVariable.VerilogLeft m l ->
+  execution_of_valuation TaggedVariable.VerilogLeft m
+    (valuation_of_executions m e1 e2) =( l )= e1.
+Proof.
+  unfold execution_of_valuation, valuation_of_executions.
+  (* intros Hdefined Hexists var Hvar_in. *)
+  intros Hdefined Hmatch var Hvar_in.
+  pose proof Hvar_in as H.
+  apply Hmatch in H. destruct H as [smtName HsmtName].
+  rewrite HsmtName.
+  rewrite VerilogSMTBijection.bij_wf in HsmtName.
+  rewrite HsmtName.
+  apply Hdefined in Hvar_in. destruct Hvar_in as [bv Hbv].
+  rewrite Hbv, XBV.xbv_bv_inverse.
+  autodestruct; [|contradiction].
+  rewrite <- eq_rect_eq.
+  reflexivity.
+Qed.
+
+Lemma execution_of_valuation_right_match_on (m : VerilogSMTBijection.t) e1 e2 l :
+  RegisterState.defined_value_for (fun var => In var l) e2 ->
+  match_map_vars TaggedVariable.VerilogRight m l ->
+  execution_of_valuation TaggedVariable.VerilogRight m
+    (valuation_of_executions m e1 e2) =( l )= e2.
+Proof.
+  unfold execution_of_valuation, valuation_of_executions.
+  (* intros Hdefined Hexists var Hvar_in. *)
+  intros Hdefined Hmatch var Hvar_in.
+  pose proof Hvar_in as H.
+  apply Hmatch in H. destruct H as [smtName HsmtName].
+  rewrite HsmtName.
+  rewrite VerilogSMTBijection.bij_wf in HsmtName.
+  rewrite HsmtName.
+  apply Hdefined in Hvar_in. destruct Hvar_in as [bv Hbv].
+  rewrite Hbv, XBV.xbv_bv_inverse.
+  autodestruct; [|contradiction].
+  rewrite <- eq_rect_eq.
+  reflexivity.
+Qed.
+
+Definition verilog_smt_match_on_name (regs : RegisterState.t) (ρ : SMTLib.valuation) var smtName : Prop :=
+  regs var = XBV.from_bv (ρ (SMTLib.Sort_BitVec (Verilog.varType var)) smtName).
+    
+Definition verilog_smt_match_states_partial
+  (cond : Verilog.variable -> Prop)
+  (tag : TaggedVariable.Tag)
+  (m : VerilogSMTBijection.t)
+  (regs : RegisterState.t)
+  (ρ : SMTLib.valuation) : Prop :=
+  forall var,
+    cond var ->
+    exists smtName,
+      m (tag, var) = Some smtName
+      /\ verilog_smt_match_on_name regs ρ var smtName.
+
+(* Might not be needed *)
+Global Instance verilog_smt_match_states_partial_proper :
+  Proper
+    (pointwise_relation Verilog.variable iff ==> eq ==> eq ==> eq ==> eq ==> iff)
+    verilog_smt_match_states_partial.
+Proof.
+  repeat intro. subst.
+  crush.
+Qed.
+
+Global Instance verilog_smt_match_states_partial_impl_proper :
+  Proper
+    (pointwise_relation Verilog.variable Basics.impl ==> eq ==> eq ==> eq ==> eq ==> Basics.flip Basics.impl)
+    verilog_smt_match_states_partial.
+Proof.
+  repeat intro. subst.
+  crush.
+Qed.
+
+Lemma verilog_smt_match_states_execution_of_valuation_same tag (m : VerilogSMTBijection.t) ρ :
+  verilog_smt_match_states_partial (fun var => exists smtName, m (tag, var) = Some smtName) tag m (execution_of_valuation tag m ρ) ρ.
+Proof.
+  intros Hhas_var.
+  unfold verilog_smt_match_states_partial, execution_of_valuation.
+  intros [smtName HsmtName].
+  exists smtName. split; [eassumption|].
+  unfold verilog_smt_match_on_name.
+  rewrite HsmtName.
+  reflexivity.
+Qed.
+
+Lemma verilog_smt_match_states_partial_impl P1 P2 tag m regs ρ :
+  (forall x, P2 x -> P1 x) ->
+  verilog_smt_match_states_partial P1 tag m regs ρ ->
+  verilog_smt_match_states_partial P2 tag m regs ρ.
+Proof. crush. Qed.
+
+Lemma verilog_smt_match_states_partial_set_reg_out C tag m r ρ var val :
+  ~ C var ->
+  verilog_smt_match_states_partial C tag m (RegisterState.set_reg var val r) ρ <->
+  verilog_smt_match_states_partial C tag m r ρ.
+Proof.
+  intro Hcond1.
+  unfold verilog_smt_match_states_partial.
+  unfold verilog_smt_match_on_name in *.
+  split; intros H * Hcond2.
+  - destruct (dec (var0 = var)).
+    + subst. contradiction.
+    + insterU H. destruct H as [smtName [? Hverilogval]].
+      econstructor. split. { eassumption. }
+      rewrite RegisterState.set_reg_get_out in Hverilogval by congruence.
+      assumption.
+  - destruct (dec (var0 = var)).
+    + subst. contradiction.
+    + insterU H. destruct H as [smtName [? Hverilogval]].
+      econstructor. split. { eassumption. }
+      rewrite RegisterState.set_reg_get_out by congruence.
+      assumption.
+Qed.
+
+Lemma verilog_smt_match_states_partial_split C1 C2 C3 tag m reg ρ :
+  (forall var, C3 var -> C1 var \/ C2 var) ->
+  verilog_smt_match_states_partial C1 tag m reg ρ ->
+  verilog_smt_match_states_partial C2 tag m reg ρ ->
+  verilog_smt_match_states_partial C3 tag m reg ρ.
+Proof.
+  unfold verilog_smt_match_states_partial.
+  intros Himpl H1 H2 * HC3.
+  apply Himpl in HC3.
+  destruct HC3; eauto.
+Qed.
+
+Lemma verilog_smt_match_states_partial_split_iff C1 C2 tag m reg ρ :
+  verilog_smt_match_states_partial (fun var => C1 var \/ C2 var) tag m reg ρ <->
+    (verilog_smt_match_states_partial C1 tag m reg ρ
+     /\ verilog_smt_match_states_partial C2 tag m reg ρ).
+Proof. unfold verilog_smt_match_states_partial. crush. Qed.
+
+Lemma verilog_smt_match_states_partial_set_reg_elim C tag (m : VerilogSMTBijection.t) regs ρ var bv :
+  (exists smtName,
+      m (tag, var) = Some smtName /\ ρ (SMTLib.Sort_BitVec (Verilog.varType var)) smtName = bv) ->
+  verilog_smt_match_states_partial C tag m regs ρ ->
+  verilog_smt_match_states_partial C tag m (RegisterState.set_reg var (XBV.from_bv bv) regs) ρ.
+Proof.
+  unfold verilog_smt_match_states_partial.
+  unfold verilog_smt_match_on_name.
+  intros Hvar Hrest *.
+  destruct (dec (var0 = var)); intros Hcond.
+  - subst.
+    insterU Hvar. destruct Hvar as [? [? ?]].
+    insterU Hrest. destruct Hrest as [? [? ?]].
+    replace x0 with x in * by congruence.
+    repeat econstructor; try eassumption; expect 1.
+    rewrite RegisterState.set_reg_get_in.
+    repeat f_equal.
+    congruence.
+  - insterU Hvar. destruct Hvar as [? [? ?]].
+    insterU Hrest. destruct Hrest as [? [? ?]].
+    repeat econstructor; try eassumption; expect 1.
+    rewrite RegisterState.set_reg_get_out; eauto.
+Qed.
+
+Lemma verilog_smt_match_states_partial_change_regs C tag m r1 r2 ρ :
+  (forall var, C var -> r1 var = r2 var) ->
+  verilog_smt_match_states_partial C tag m r1 ρ ->
+  verilog_smt_match_states_partial C tag m r2 ρ.
+Proof.
+  unfold verilog_smt_match_states_partial.
+  intros Hsame Hmatch1 * Hcond.
+  insterU Hsame. insterU Hcond. insterU Hmatch1.
+  destruct Hmatch1 as [smtName [? ?]].
+  exists smtName.
+  split. { eassumption. }
+  unfold verilog_smt_match_on_name in *.
+  congruence.
+Qed.
+
+Ltac unpack_verilog_smt_match_states_partial :=
+  repeat match goal with
+    | [ H: verilog_smt_match_states_partial (fun _ => _ \/ _) _ _ _ _ |- _ ] =>
+        apply verilog_smt_match_states_partial_split_iff in H;
+        destruct H
+    | [ H: verilog_smt_match_states_partial (fun _ => List.In _ (_ ++ _)) _ _ _ _ |- _ ] =>
+        setoid_rewrite List.in_app_iff in H
+    | [ |- verilog_smt_match_states_partial (fun _ => List.In _ (_ ++ _)) _ _ _ _ ] =>
+        setoid_rewrite List.in_app_iff
+    | [ |- verilog_smt_match_states_partial (fun _ => _ \/ _) _ _ _ _ ] =>
+        apply verilog_smt_match_states_partial_split_iff; split
+    end.
+
+Lemma verilog_smt_match_states_partial_defined_value_for C tag m regs ρ :
+  verilog_smt_match_states_partial C tag m regs ρ ->
+  RegisterState.defined_value_for C regs.
+Proof.
+  unfold verilog_smt_match_states_partial, verilog_smt_match_on_name, RegisterState.defined_value_for.
+  intros Hmatch * Hcond.
+  edestruct Hmatch as [? [? ?]]; eauto.
+Qed.
+
+Lemma verilog_smt_match_states_partial_execution_match_on C tag m ρ e :
+    verilog_smt_match_states_partial C tag m e ρ ->
+    e ={ C }= execution_of_valuation tag m ρ.
+Proof.
+  unfold verilog_smt_match_states_partial, "_ ={ _ }= _".
+  unfold verilog_smt_match_on_name.
+  intros H var Hvar.
+  edestruct H as [? [H1 H2]]; [eauto|].
+  unfold execution_of_valuation.
+  rewrite H1. assumption.
+Qed.
+
+Lemma verilog_smt_match_states_partial_execution_defined_value_for C tag m ρ e :
+    verilog_smt_match_states_partial C tag m e ρ ->
+    RegisterState.defined_value_for C e.
+Proof.
+  unfold verilog_smt_match_states_partial, RegisterState.defined_value_for.
+  intros H var Hvar.
+  edestruct H as [? [H1 H2]]; [eauto|].
+  inv H2. eauto.
+Qed.
+
+Lemma execution_of_valuation_inv tag m ρ var bv :
+  execution_of_valuation tag m ρ var = XBV.from_bv bv ->
+  exists smtName,
+    m (tag, var) = Some smtName /\
+    ρ (SMTLib.Sort_BitVec (Verilog.varType var)) smtName = bv .
+Proof.
+  unfold execution_of_valuation.
+  intros H.
+  (* We don't know that var is in m. We could have added it directly
+  as an assumption, but we can also deduce it from the fact that the
+  value of the var in e is defined. This is only possible, however, if
+  the var is not zero-width (because zero-width Xs are
+  indistinguishable from zero-width 0/1s). This lemma is why we have
+  added varTypeWf into verilog variables *)
+
+  destruct (m (tag, var)).
+  - apply XBV.from_bv_injective in H.
     eauto.
-  Qed.
+  - exfalso.
+    apply f_equal with (f:=XBV.to_bv) in H.
+    autorewrite with xbv in H.
+    rewrite XBV.exes_to_bv in H by apply Verilog.varTypeWf.
+    discriminate.
+Qed.
 
-  Definition valuation_of_executions (m : VerilogSMTBijection.t) (e1 e2 : execution) : SMTLib.valuation :=
-    fun s smtName =>
-      match s as s' return SMTLib.interp_sort s' with
-      | SMTLib.Sort_Bool => default _
-      | SMTLib.Sort_BitVec w => 
-        match bij_inverse m smtName with
-	| None => default _
-	| Some (tag, verilogVar) =>
-	  match dec (Verilog.varType verilogVar = w) with
-	  | right _ => default _
-	  | left E =>
-            let e :=
-              match tag with
-              | TaggedVariable.VerilogLeft => e1
-              | TaggedVariable.VerilogRight => e2
-              end
-            in
-              match XBV.to_bv (e verilogVar) with
-              (* TODO: Fix handling of Xs *)
-              | None => default _
-              | Some val => rew E in val
-              end
-	  end
-	end
-      end.
+Lemma execution_match_on_verilog_smt_match_states_partial C tag m ρ e :
+    RegisterState.defined_value_for C e ->
+    e ={ C }= (execution_of_valuation tag m ρ) ->
+    verilog_smt_match_states_partial C tag m e ρ.
+Proof.
+  unfold RegisterState.defined_value_for, verilog_smt_match_states_partial, "_ =( _ )= _".
+  intros Hdefined Heq var Hvar.
+  insterU Hdefined. insterU Heq.
+  destruct Hdefined as [bv Hbv]. 
+  unfold verilog_smt_match_on_name in *.
+  unfold execution_of_valuation in *.
 
-  Lemma execution_of_valuation_left_match_on (m : VerilogSMTBijection.t) e1 e2 l :
-    RegisterState.defined_value_for (fun var => In var l) e1 ->
-    SMT.match_map_vars TaggedVariable.VerilogLeft m l ->
-    SMT.execution_of_valuation TaggedVariable.VerilogLeft m
-      (SMT.valuation_of_executions m e1 e2) =( l )= e1.
-  Proof.
-    unfold SMT.execution_of_valuation, SMT.valuation_of_executions.
-    (* intros Hdefined Hexists var Hvar_in. *)
-    intros Hdefined Hmatch var Hvar_in.
-    pose proof Hvar_in as H.
-    apply Hmatch in H. destruct H as [smtName HsmtName].
-    rewrite HsmtName.
-    rewrite VerilogSMTBijection.bij_wf in HsmtName.
-    rewrite HsmtName.
-    apply Hdefined in Hvar_in. destruct Hvar_in as [bv Hbv].
-    rewrite Hbv, XBV.xbv_bv_inverse.
-    autodestruct; [|contradiction].
-    rewrite <- eq_rect_eq.
-    reflexivity.
-  Qed.
+  (* TODO: Use execution_of_valuation_inv instead. *)
 
-  Lemma execution_of_valuation_right_match_on (m : VerilogSMTBijection.t) e1 e2 l :
-    RegisterState.defined_value_for (fun var => In var l) e2 ->
-    SMT.match_map_vars TaggedVariable.VerilogRight m l ->
-    SMT.execution_of_valuation TaggedVariable.VerilogRight m
-      (SMT.valuation_of_executions m e1 e2) =( l )= e2.
-  Proof.
-    unfold SMT.execution_of_valuation, SMT.valuation_of_executions.
-    (* intros Hdefined Hexists var Hvar_in. *)
-    intros Hdefined Hmatch var Hvar_in.
-    pose proof Hvar_in as H.
-    apply Hmatch in H. destruct H as [smtName HsmtName].
-    rewrite HsmtName.
-    rewrite VerilogSMTBijection.bij_wf in HsmtName.
-    rewrite HsmtName.
-    apply Hdefined in Hvar_in. destruct Hvar_in as [bv Hbv].
-    rewrite Hbv, XBV.xbv_bv_inverse.
-    autodestruct; [|contradiction].
-    rewrite <- eq_rect_eq.
-    reflexivity.
-  Qed.
-End SMT.
+  (* We don't know that var is in m. We could have added it directly
+  as an assumption, but we can also deduce it from the fact that the
+  value of the var in e is defined. This is only possible, however, if
+  the var is not zero-width (because zero-width Xs are
+  indistinguishable from zero-width 0/1s). This lemma is why we have
+  added varTypeWf into verilog variables *)
+
+  destruct (m (tag, var)); [solve [eauto]|].
+  exfalso.
+  rewrite Hbv in Heq. clear Hbv.
+  apply f_equal with (f:=XBV.to_bv) in Heq.
+  autorewrite with xbv in Heq.
+  rewrite XBV.exes_to_bv in Heq by apply Verilog.varTypeWf.
+  discriminate.
+Qed.
